DY/Bytes/AttackerKnowledge.lean
@@ -8,6 +8,7 @@ module
 public import DY.Kleene
 public import DY.Bytes.Basic
 public import DY.Trace.Basic
+public import DY.Trace.BaseAttackerKnowledge
 
 namespace DY
 
@@ -157,16 +158,12 @@ where
 
 end AttackerKnowledge
 
--- TODO
-public
-opaque Trace.MessageSent (tr: Trace α) (b: Bytes): Prop
-
 @[expose]
 public
-def Bytes.AttackerKnows.baseKnowledge (tr: Trace α): SubAttackerKnowledge BytesF :=
-  SubAttackerKnowledge.fromPred tr.MessageSent
+def Bytes.AttackerKnows.baseKnowledge [ExecTraceTypes] [BaseAttackerKnowledge] (tr: ExecTrace): SubAttackerKnowledge BytesF :=
+  SubAttackerKnowledge.fromPred tr.BaseAttackerKnows
 
-def Bytes.AttackerKnows.attackerKnowledge [AttackerKnowledge] (tr: Trace α): SubAttackerKnowledge BytesF :=
+def Bytes.AttackerKnows.attackerKnowledge [ExecTraceTypes] [BaseAttackerKnowledge] [AttackerKnowledge] (tr: ExecTrace): SubAttackerKnowledge BytesF :=
   SubAttackerKnowledge.combine' (fun (id: Fin 2) =>
     match id with
     | 0 => AttackerKnowledge.attackerKnowledge
@@ -174,16 +171,17 @@ def Bytes.AttackerKnows.attackerKnowledge [AttackerKnowledge] (tr: Trace α): Su
   )
 
 public
-def Bytes.AttackerKnows [AttackerKnowledge] (b: Bytes) (tr: Trace α): Prop :=
+def Bytes.AttackerKnows [ExecTraceTypes] [BaseAttackerKnowledge] [AttackerKnowledge] (b: Bytes) (tr: ExecTrace): Prop :=
   Kleene.mkWeakestFixpoint ((Bytes.AttackerKnows.attackerKnowledge tr).pred) b
 
 def Bytes.AttackerKnows.attackerKnow.prove
-  [AttackerKnowledge]
+  [ExecTraceTypes]
+  [BaseAttackerKnowledge] [AttackerKnowledge]
   {SubF: Type → Type}
   (att: SubAttackerKnowledge SubF)
   [inst: AttackerKnowledge.Has att]
   (p: Bytes → Prop)
-  (b: Bytes) (tr: Trace α)
+  (b: Bytes) (tr: ExecTrace)
   : att.pred p b → (Bytes.AttackerKnows.attackerKnowledge tr).pred p b
 := by
   unfold Bytes.AttackerKnows.attackerKnowledge SubAttackerKnowledge.combine' Kleene.combine
@@ -196,11 +194,12 @@ def Bytes.AttackerKnows.attackerKnow.prove
 -/
 public
 theorem Bytes.AttackerKnows.prove
-  [AttackerKnowledge]
+  [ExecTraceTypes]
+  [BaseAttackerKnowledge] [AttackerKnowledge]
   {SubF: Type → Type}
   (att: SubAttackerKnowledge SubF)
   [AttackerKnowledge.Has att]
-  (b: Bytes) (tr: Trace α)
+  (b: Bytes) (tr: ExecTrace)
   : att.pred (Bytes.AttackerKnows · tr) b →
     Bytes.AttackerKnows b tr
 := by
@@ -257,9 +256,10 @@ theorem SubAttackerKnowledge.combine.implies
 
 public
 theorem Bytes.AttackerKnows.is_least_fixpoint
-  [AttackerKnowledge]
+  [ExecTraceTypes]
+  [BaseAttackerKnowledge] [AttackerKnowledge]
   (pred: Bytes → Prop)
-  (b: Bytes) (tr: Trace α)
+  (b: Bytes) (tr: ExecTrace)
   (pf1: SubAttackerKnowledge.Implies AttackerKnowledge.attackerKnowledge pred)
   (pf2: SubAttackerKnowledge.Implies (Bytes.AttackerKnows.baseKnowledge tr) pred)
   : Bytes.AttackerKnows b tr →
