DY/EquationalTheory/DiffieHellman.lean
@@ -199,11 +199,12 @@ def attackerKnowledge: SubAttackerKnowledge SubF :=
 instance: AttackerKnowledge.HasStep attKnowsDhPk attackerKnowledge := inferInstanceAs (AttackerKnowledge.HasStep (attackerKnowledge.internal 0) (SubAttackerKnowledge.combine' attackerKnowledge.internal))
 instance: AttackerKnowledge.HasStep attKnowsDh attackerKnowledge := inferInstanceAs (AttackerKnowledge.HasStep (attackerKnowledge.internal 1) (SubAttackerKnowledge.combine' attackerKnowledge.internal))
 
+variable [ExecTraceTypes] [BaseAttackerKnowledge]
 variable [AttackerKnowledge] [AttackerKnowledge.Has attackerKnowledge]
 
 public
 theorem attacker_knows_dh_pk
-  (sk: Bytes) (tr: Trace α)
+  (sk: Bytes) (tr: ExecTrace)
   : sk.AttackerKnows tr →
     (dh_pk sk).AttackerKnows tr
 := by
@@ -214,7 +215,7 @@ theorem attacker_knows_dh_pk
 
 public
 theorem attacker_knows_dh
-  (pk sk: Bytes) (tr: Trace α)
+  (pk sk: Bytes) (tr: ExecTrace)
   : pk.AttackerKnows tr →
     sk.AttackerKnows tr →
     (dh pk sk).AttackerKnows tr
