DY/Trace.lean
@@ -1,6 +1,7 @@
 module
 
 public import DY.Trace.Basic
-public import DY.Trace.AttackerKnowledge
+public import DY.Trace.BaseAttackerKnowledge
 public import DY.Trace.Invariant
+public import DY.Trace.BaseAttackerKnowledgeTheorem
 public import DY.Trace.Manipulation
