DY/Trace/BaseAttackerKnowledge.lean
@@ -1,0 +1,42 @@
+module
+
+public import DY.Bytes.Basic
+public import DY.Trace.Basic
+import all DY.Trace.Basic
+
+namespace DY
+
+public
+structure EntryBaseAttackerKnowledge [BytesFunctor] [ExecTraceTypes] (ExecEntryT: Type) where
+  attackerKnows: ExecTrace → ExecEntryT → Bytes → Prop
+
+public
+class BaseAttackerKnowledge [BytesFunctor] [ExecTraceTypes] where
+  attackerKnows: ∀ id, EntryBaseAttackerKnowledge (ExecTraceTypes.entries id)
+
+public
+def Trace.BaseAttackerKnows
+  [BytesFunctor] [ExecTraceTypes] [BaseAttackerKnowledge]
+  (tr: ExecTrace) (b: Bytes)
+  : Prop
+:=
+  match tr with
+  | .nil => False
+  | .snoc trBefore entry =>
+    (BaseAttackerKnowledge.attackerKnows entry.id).attackerKnows trBefore entry.entry b ∨
+    Trace.BaseAttackerKnows trBefore b
+
+public
+def Trace.prove_BaseAttackerKnows
+  [BytesFunctor] [ExecTraceTypes] [BaseAttackerKnowledge]
+  (tr: ExecTrace) (b: Bytes)
+  (time: Nat) (h_time: time < tr.length)
+  : (BaseAttackerKnowledge.attackerKnows (tr.at time h_time).id).attackerKnows (tr.prefix time) (tr.at time h_time).entry b
+    → Trace.BaseAttackerKnows tr b
+:= by
+  induction tr
+  · grind [Trace.length]
+  simp_all only [Trace.at, Trace.prefix, Trace.length, Trace.BaseAttackerKnows]
+  grind
+
+end DY
