DY/Trace/BaseAttackerKnowledgeTheorem.lean
@@ -1,0 +1,57 @@
+module
+
+public import DY.Bytes.Basic
+public import DY.Bytes.Invariants
+public import DY.Trace.Basic
+public import DY.Trace.Invariant
+public import DY.Trace.BaseAttackerKnowledge
+import all DY.Trace.Invariant
+import all DY.Trace.BaseAttackerKnowledge
+
+namespace DY
+
+public
+structure EntryBaseAttackerKnowledgeTheorem
+  [TraceInvariant]
+  [BytesFunctor] [BytesInvariants]
+  {ExecEntryT: Type} {ProofEntryT: Type}
+  {func: ProofEntryFun ExecEntryT ProofEntryT}
+  (inv: TraceEntryInvariant func)
+  [TraceInvariant.Has inv]
+  (att: EntryBaseAttackerKnowledge ExecEntryT)
+where
+  pf: ∀ trBefore entry (b: Bytes),
+    inv.invariant trBefore entry →
+    att.attackerKnows trBefore.erase (func.erase entry) b →
+    b.Publishable trBefore -- could also be `b.Publishable (trBefore.append entry)` if needed
+
+public
+class BaseAttackerKnowledgeTheorem
+  [TraceInvariant]
+  [BytesFunctor] [BytesInvariants]
+  [BaseAttackerKnowledge]
+where
+  pfs: ∀ id, EntryBaseAttackerKnowledgeTheorem (TraceInvariant.invs id) (BaseAttackerKnowledge.attackerKnows id)
+
+public
+theorem Trace.BaseAttackerKnows_implies_Publishable
+  [TraceInvariant]
+  [BytesFunctor] [BytesInvariants] [BytesInvariantsProofs]
+  [BaseAttackerKnowledge] [BaseAttackerKnowledgeTheorem]
+  (tr: ProofTrace) (b: Bytes)
+  : Trace.Invariant tr →
+    Trace.BaseAttackerKnows tr.erase b →
+    b.Publishable tr
+:= by
+  induction tr
+  · simp [Trace.BaseAttackerKnows, Trace.erase]
+  rename_i trBefore entry ih
+  have h_le: trBefore ≤ trBefore.snoc entry := by apply Trace.le.extend; apply Trace.le.equal
+  simp only [Trace.Invariant, Trace.BaseAttackerKnows, Trace.erase]
+  intro h_inv h_att
+  cases h_att
+  · have := (BaseAttackerKnowledgeTheorem.pfs entry.id).pf trBefore entry.entry b (by grind [ProofTrace.Entry.Invariant]) (by grind [ProofTrace.Entry.erase])
+    grind
+  · grind
+
+end DY
